{
 "cells": [
  {
   "cell_type": "markdown",
   "id": "6yBntbwezbkJ",
   "metadata": {
    "id": "6yBntbwezbkJ"
   },
   "source": [
    "## Mathematics Behind Multinomial Logistic Regression"
   ]
  },
  {
   "cell_type": "markdown",
   "id": "96fec292",
   "metadata": {
    "id": "96fec292"
   },
   "source": [
    "### Formulating the Problem\n",
    "Suppose there are 3 classes in the response variable. Let us denote the classes by Class 1, Class 2 and Class 3.  \n",
    "\n",
    "We set,\n",
    "$$\n",
    "P(Y = 1|\\vec{x}_i) = \\frac{e^{\\vec{x}_i^T.\\vec{\\beta}_1}}{1+e^{\\vec{x}_i^T.\\vec{\\beta}_1}+e^{\\vec{x}_i^T.\\vec{\\beta}_2}}, \\ \\ \n",
    "P(Y = 2|\\vec{x}_i) = \\frac{e^{\\vec{x}_i^T.\\vec{\\beta}_2}}{1+e^{\\vec{x}_i^T.\\vec{\\beta}_1}+e^{\\vec{x}_i^T.\\vec{\\beta}_2}} \n",
    "$$\n",
    "\n",
    "\n",
    "As a result,\n",
    "$$\n",
    "\\begin{aligned}\n",
    "P(Y = 3|\\vec{x}_i) \n",
    " &= 1 \\ - \\ P(Y = 1|\\vec{x}_i) - P(Y = 2|\\vec{x}_i) \\\\\n",
    " \\\\\n",
    " &= 1 - \\frac{e^{\\vec{x}_i^T.\\vec{\\beta}_1}}{1+e^{\\vec{x}_i^T.\\vec{\\beta}_1}+e^{\\vec{x}_i^T.\\vec{\\beta}_2}}-\\frac{e^{\\vec{x}_i^T.\\vec{\\beta}_2}}{1+e^{\\vec{x}_i^T.\\vec{\\beta}_1}+e^{\\vec{x}_i^T.\\vec{\\beta}_2}} \\\\\n",
    " \\\\\n",
    " &= \\frac{1}{1+e^{\\vec{x}_i^T.\\vec{\\beta}_1}+e^{\\vec{x}_i^T.\\vec{\\beta}_2}}\n",
    "\\end{aligned}\n",
    "$$\n",
    "\n",
    "### Likelihood and Log-Likelihood\n",
    "So, likelihood,\n",
    "$$\\begin{aligned}\n",
    "L &= \\prod_{i=1}^n \\left[P(y_i = 1 \\ \\ | \\ \\ \\vec{x}_i)^{I(y_i=1)}\\right].\\left[P(y_i = 2 \\ \\ | \\ \\ \\vec{x}_i)^{I(y_i=2)}\\right].\\left[P(y_i =  3 \\ \\ | \\ \\ \\vec{x}_i)^{I(y_i=3)}\\right] \\\\\n",
    " &= \\prod_{i=1}^n \\left[\\frac{e^{\\vec{x}_i^T.\\vec{\\beta}_1}}{1+e^{\\vec{x}_i^T.\\vec{\\beta}_1}+e^{\\vec{x}_i^T.\\vec{\\beta}_2}}\\right]^{I(y_i=1)}\\left[\\frac{e^{\\vec{x}_i^T.\\vec{\\beta}_2}}{1+e^{\\vec{x}_i^T.\\vec{\\beta}_1}+e^{\\vec{x}_i^T.\\vec{\\beta}_2}}\\right]^{I(y_i=2)}\\left[\\frac{1}{1+e^{\\vec{x}_i^T.\\vec{\\beta}_1}+e^{\\vec{x}_i^T.\\vec{\\beta}_2}}\\right]^{I(y_i=3)} \\\\\n",
    " &= \\prod_{i=1}^n \\ e^{\\vec{x}_i^T.\\vec{\\beta}_1.I(y_i=1)} \\ . \\ e^{\\vec{x}_i^T.\\vec{\\beta}_2.I(y_i=2)}.\\left[\\frac{1}{1+e^{\\vec{x}_i^T.\\vec{\\beta}_1}+e^{\\vec{x}_i^T.\\vec{\\beta}_2}}\\right]^{[I(y_i=1) + I(y_i=2) + I(y_i=3)]} \\\\\n",
    " &= \\prod_{i=1}^n \\ e^{\\vec{x}_i^T.\\vec{\\beta}_1.I(y_i=1)} \\ . \\ e^{\\vec{x}_i^T.\\vec{\\beta}_2.I(y_i=2)}.\\frac{1}{1+e^{\\vec{x}_i^T.\\vec{\\beta}_1}+e^{\\vec{x}_i^T.\\vec{\\beta}_2}}\n",
    "\\end{aligned}\n",
    "$$\n",
    "\n",
    "\n",
    "Last equality holds as $I(y_i=1) + I(y_i=2) + I(y_i=3) = 1$.\n",
    "\n",
    "So,\n",
    "$$\\begin{aligned}\n",
    "log L &= log \\ \\prod_{i=1}^n \\ e^{\\vec{x}_i^T.\\vec{\\beta}_1.I(y_i=1)} \\ . \\ e^{\\vec{x}_i^T.\\vec{\\beta}_2.I(y_i=2)}.\\frac{1}{1+e^{\\vec{x}_i^T.\\vec{\\beta}_1}+e^{\\vec{x}_i^T.\\vec{\\beta}_2}} \\\\\n",
    " &= \\sum_{i=1}^nlog\\left[e^{\\vec{x}_i^T.\\vec{\\beta}_1.I(y_i=1)}\\right] + log\\left[e^{\\vec{x}_i^T.\\vec{\\beta}_2.I(y_i=2)}\\right] - log\\left[1+e^{\\vec{x}_i^T.\\vec{\\beta}_1}+e^{\\vec{x}_i^T.\\vec{\\beta}_2}\\right] \\\\\n",
    " &= \\sum_{i=1}^n I(y_i=1).\\vec{x}_i^T.\\vec{\\beta}_1 + \\sum_{i=1}^nI(y_i=2).\\vec{x}_i^T.\\vec{\\beta}_2 - \\sum_{i=1}^nlog\\left[1+e^{\\vec{x}_i^T.\\vec{\\beta}_1}+e^{\\vec{x}_i^T.\\vec{\\beta}_2}\\right]\n",
    "\\end{aligned}$$\n",
    "\n",
    "### Deriving the First Derivative\n",
    "First derivative,\n",
    "$$\\begin{aligned}\\frac{\\partial}{\\partial \\vec{\\beta}}log L &= \\begin{pmatrix}\\frac{\\partial}{\\partial \\vec{\\beta}_1}log L \\\\ \n",
    "\\frac{\\partial}{\\partial \\vec{\\beta}_2}log L \\end{pmatrix}\n",
    "\\end{aligned}$$\n",
    "\n",
    "Now,\n",
    "$$\\begin{aligned}\n",
    "\\frac{\\partial}{\\partial \\vec{\\beta_1}}log L &= \\frac{\\partial}{\\partial \\vec{\\beta_1}} \\left[\\sum_{i=1}^n I(y_i=1).\\vec{x}_i^T.\\vec{\\beta}_1 + \\sum_{i=1}^nI(y_i=2).\\vec{x}_i^T.\\vec{\\beta}_2 - \\sum_{i=1}^nlog\\left[1+e^{\\vec{x}_i^T.\\vec{\\beta}_1}+e^{\\vec{x}_i^T.\\vec{\\beta}_2}\\right]\\right] \\\\ \n",
    " &= \\sum_{i=1}^n I(y_i=1).\\vec{x}_i \\ + \\ 0  \\ - \\ \\sum_{i=1}^n\\frac{1}{1+e^{\\vec{x}_i^T.\\vec{\\beta}_1}+e^{\\vec{x}_i^T.\\vec{\\beta}_2}}.e^{\\vec{x}_i^T.\\vec{\\beta}_1}.\\vec{x}_i \\\\ \n",
    " &= \\sum_{i=1}^n I(y_i=1) \\ . \\ \\vec{x}_i \\ \\ - \\ \\ \\sum_{i=1}^n P(y_i=1|\\vec{x}_i) \\ . \\ \\vec{x}_i \\\\ \n",
    " &= \\sum_{i=1}^n \\left[ \\ \\ I(y_i=1) - P(y_i=1|\\vec{x}_i) \\ \\ \\right].\\vec{x}_i\n",
    "\\end{aligned}\n",
    "$$\n",
    "\n",
    "Similarly,\n",
    "$$\\frac{\\partial}{\\partial \\vec{\\beta_2}}log L = \\sum_{i=1}^n \\left[ \\ \\ I(y_i=2) - P(y_i=2|\\vec{x}_i) \\ \\ \\right].\\vec{x}_i$$\n",
    "\n",
    "So,\n",
    "$$\\begin{aligned}\n",
    "\\frac{\\partial}{\\partial \\vec{\\beta}}log L &= \\begin{pmatrix}\\frac{\\partial}{\\partial \\vec{\\beta}_1}log L \\\\ \n",
    "\\frac{\\partial}{\\partial \\vec{\\beta}_2}log L \\end{pmatrix} \\\\ \n",
    " \\\\\n",
    " &= \\begin{bmatrix}\\sum_{i=1}^n \\left[ \\ \\ I(y_i=1) - P(y_i=1|\\vec{x}_i) \\ \\ \\right].\\vec{x}_i \\\\ \n",
    " \\sum_{i=1}^n \\left[ \\ \\ I(y_i=2) - P(y_i=2|\\vec{x}_i) \\ \\ \\right].\\vec{x}_i\\end{bmatrix} \\\\ \n",
    " \\\\ \n",
    " &= \\sum_{i=1}^n \\begin{bmatrix} \\left[ \\ \\ I(y_i=1) - P(y_i=1|\\vec{x}_i) \\ \\ \\right].\\vec{x}_i \\\\ \n",
    " \\left[ \\ \\ I(y_i=2) - P(y_i=2|\\vec{x}_i) \\ \\ \\right].\\vec{x}_i\\end{bmatrix} \\\\ \n",
    " \\\\ \n",
    " &= \\sum_{i=1}^n \\begin{bmatrix}\\ \\ I(y_i=1) - P(y_i=1|\\vec{x}_i) \\ \\  \\\\ \n",
    " \\ \\ I(y_i=2) - P(y_i=2|\\vec{x}_i) \\ \\ \\end{bmatrix} \\otimes \\ \\vec{x}_i\n",
    "\\end{aligned}$$\n",
    "\n",
    "Here, $\\ \\ \\ \\vec{\\beta}^T = \\left(\\vec{\\beta}_1^T \\ \\ \\ \\vec{\\beta}_2^T\\right)$ and $\\ \\ \\otimes$ is **Kronecker product**.\n",
    "\n",
    "### Deriving the Hessian Matrix\n",
    "Hessian matrix, \n",
    "$$\\begin{aligned}\n",
    "H &= \\frac{\\partial}{\\partial \\vec{\\beta}}\\left[ \\frac{\\partial}{\\partial \\vec{\\beta}}log \\ L \\right]^T \\\\\n",
    " &= \\begin{bmatrix}\\frac{\\partial}{\\partial \\vec{\\beta}_1} \\left[ \\frac{\\partial}{\\partial \\vec{\\beta}}log \\ L \\right]^T \\\\ \n",
    "    \\frac{\\partial}{\\partial \\vec{\\beta}_2} \\left[ \\frac{\\partial}{\\partial \\vec{\\beta}}log \\ L \\right]^T\n",
    "    \\end{bmatrix}\n",
    "\\end{aligned}\n",
    "$$\n",
    "Now,\n",
    "$$\\begin{aligned}\n",
    "\\frac{\\partial}{\\partial \\vec{\\beta}_1} \\left[ \\frac{\\partial}{\\partial \\vec{\\beta}}log \\ L \\right]^T &= \\frac{\\partial}{\\partial \\vec{\\beta}_1} \\sum_{i=1}^n\\left[ \\ I(y_i=1) - P(y_i=1|\\vec{x}_i) \\ \\ \\ \\ I(y_i=2) - P(y_i=2|\\vec{x}_i) \\ \\right] \\otimes \\vec{x}_i^T \\\\ \n",
    " &= \\sum_{i=1}^n\\left[ \\ \\frac{\\partial}{\\partial \\vec{\\beta}_1}\\left[I(y_i=1) - P(y_i=1|\\vec{x}_i)\\right] \\ \\ \\ \\ \\ \\frac{\\partial}{\\partial \\vec{\\beta}_1}\\left[I(y_i=2) - P(y_i=2|\\vec{x}_i)\\right] \\ \\right] \\otimes \\vec{x}_i^T \\\\\n",
    " &= \\sum_{i=1}^n \\left[ \\ \\ 0 - \\frac{\\partial}{\\partial \\vec{\\beta}_1}P(y_i=1|\\vec{x}_i) \\ \\ \\ \\  0 - \\frac{\\partial}{\\partial \\vec{\\beta}_1}P(y_i=2|\\vec{x}_i) \\ \\ \\right] \\otimes \\vec{x}_i^T \\\\ \n",
    " &= -\\sum_{i=1}^n \\left[ \\ \\ \\frac{\\partial}{\\partial \\vec{\\beta}_1}P(y_i=1|\\vec{x}_i) \\ \\ \\ \\  \\frac{\\partial}{\\partial \\vec{\\beta}_1}P(y_i=2|\\vec{x}_i) \\ \\ \\right] \\otimes \\vec{x}_i^T\n",
    " \\end{aligned}$$\n",
    "\n",
    " Now,\n",
    "$$\\begin{aligned}\n",
    "\\frac{\\partial}{\\partial \\beta_{1j}} P(y_i=1|\\vec{x}_i) &= \\frac{\\partial}{\\partial \\beta_{1j}} \\frac{e^{\\vec{x}_i^T.\\vec{\\beta}_1}}{1+e^{\\vec{x}_i^T.\\vec{\\beta}_1}+e^{\\vec{x}_i^T.\\vec{\\beta}_2}} \\\\ \n",
    " \\\\\n",
    " &= \\frac{(1+e^{\\vec{x}_i^T.\\vec{\\beta}_1}+e^{\\vec{x}_i^T.\\vec{\\beta}_2}).e^{\\vec{x}_i^T.\\vec{\\beta}_1}.x_{ij} - (e^{\\vec{x}_i^T.\\vec{\\beta}_1})^2.x_{ij}}{(1+e^{\\vec{x}_i^T.\\vec{\\beta}_1}+e^{\\vec{x}_i^T.\\vec{\\beta}_2})^2} \\\\ \n",
    " \\\\\n",
    " &= \\frac{e^{\\vec{x}_i^T.\\vec{\\beta}_1}.x_{ij}}{(1+e^{\\vec{x}_i^T.\\vec{\\beta}_1}+e^{\\vec{x}_i^T.\\vec{\\beta}_2})^2}.[1+e^{\\vec{x}_i^T.\\vec{\\beta}_2}] \\\\ \n",
    " \\\\\n",
    " &= P(y_i=1|\\vec{x}_i).P(y_i\\neq1|\\vec{x}_i).x_{ij}\n",
    "\\end{aligned}$$\n",
    "\n",
    "So,\n",
    "$$\\begin{aligned}\n",
    "\\frac{\\partial}{\\partial \\vec{\\beta}_1}P(y_i=1|\\vec{x}_i) &= \n",
    "\\begin{pmatrix}\n",
    "\\frac{\\partial}{\\partial \\beta_{11}} P(y_i=1|\\vec{x}_i) \\\\ \n",
    "\\frac{\\partial}{\\partial \\beta_{12}} P(y_i=1|\\vec{x}_i) \\\\ \n",
    ". \\\\ \n",
    ". \\\\ \n",
    ". \\\\ \n",
    "\\frac{\\partial}{\\partial \\beta_{1p}} P(y_i=1|\\vec{x}_i) \\\\ \n",
    "\\end{pmatrix} \\\\ \n",
    " \\\\ \n",
    " &= \\begin{pmatrix}P(y_i=1|\\vec{x}_i).P(y_i\\neq1|\\vec{x}_i).x_{i1} \\\\ \n",
    " P(y_i=1|\\vec{x}_i).P(y_i\\neq1|\\vec{x}_i).x_{i2} \\\\ \n",
    " . \\\\ \n",
    " . \\\\ \n",
    " . \\\\ \n",
    " P(y_i=1|\\vec{x}_i).P(y_i\\neq1|\\vec{x}_i).x_{ip} \n",
    " \\end{pmatrix} \\\\ \n",
    " \\\\ \n",
    " &= P(y_i=1|\\vec{x}_i).P(y_i\\neq1|\\vec{x}_i).\\begin{pmatrix}x_{i1} \\\\ \n",
    " x_{i2} \\\\ \n",
    " x_{i3} \\\\ \n",
    " . \\\\ \n",
    " . \\\\ \n",
    " . \\\\ \n",
    " x_{ip}\n",
    " \\end{pmatrix} \\\\ \n",
    " \\\\ \n",
    " &= P(y_i=1|\\vec{x}_i).P(y_i\\neq1|\\vec{x}_i).\\vec{x}_i\n",
    "\\end{aligned}\n",
    "$$\n",
    "\n",
    "$$P(y_i=2|\\vec{x}_i) = \\frac{e^{\\vec{x}_i^T.\\vec{\\beta}_2}}{1+e^{\\vec{x}_i^T.\\vec{\\beta}_1}+e^{\\vec{x}_i^T.\\vec{\\beta}_2}}$$\n",
    "\n",
    "and,\n",
    "$$\\begin{aligned}\n",
    "\\frac{\\partial}{\\partial \\beta_{1j}} P(y_i=2|\\vec{x}_i) &= - \\frac{e^{\\vec{x}_i^T.\\vec{\\beta}_2}.e^{\\vec{x}_i^T.\\vec{\\beta}_1}.x_{ij}}{(1+e^{\\vec{x}_i^T.\\vec{\\beta}_1}+e^{\\vec{x}_i^T.\\vec{\\beta}_2})^2} \\\\ \n",
    " &= - P(y_i=1|\\vec{x}_i).P(y_i=2|\\vec{x}_i).x_{ij} \\\\ \n",
    "\\end{aligned}$$\n",
    "\n",
    "So,\n",
    "$$\\frac{\\partial}{\\partial \\vec{\\beta}_1}P(y_i=2|\\vec{x}_i) = - P(y_i=1|\\vec{x}_i).P(y_i=2|\\vec{x}_i).\\vec{x}_i$$\n",
    "\n",
    "So,\n",
    "$$\\begin{aligned}\n",
    "\\frac{\\partial}{\\partial \\vec{\\beta}_1}\\left[\\frac{\\partial}{\\partial \\vec{\\beta}}log L\\right]^T &= -\\sum_{i=1}^n \\left[ \\ \\ \\frac{\\partial}{\\partial \\vec{\\beta}_1}P(y_i=1|\\vec{x}_i) \\ \\ \\ \\  \\frac{\\partial}{\\partial \\vec{\\beta}_1}P(y_i=2|\\vec{x}_i) \\ \\ \\right] \\otimes \\vec{x}_i^T \\\\ \n",
    " &= -\\sum_{i=1}^n \\left[P(y_i=1|\\vec{x}_i).P(y_i\\neq1|\\vec{x}_i).\\vec{x}_i \\ \\ \\ \\  - P(y_i=1|\\vec{x}_i).P(y_i=2|\\vec{x}_i).\\vec{x}_i\\right] \\otimes \\vec{x}_i^T \\\\ \n",
    " &= -\\sum_{i=1}^n\\left[P(y_i=1|\\vec{x}_i).P(y_i\\neq1|\\vec{x}_i) \\ \\ \\ \\ - P(y_i=1|\\vec{x}_i).P(y_i=2|\\vec{x}_i)\\right]\\otimes\\vec{x}_i\\otimes\\vec{x}_i^T \\\\ \n",
    " &= -\\sum_{i=1}^n\\left[P(y_i=1|\\vec{x}_i).P(y_i\\neq1|\\vec{x}_i) \\ \\ \\ \\ - P(y_i=1|\\vec{x}_i).P(y_i=2|\\vec{x}_i)\\right]\\otimes\\vec{x}_i.\\vec{x}_i^T\\end{aligned}$$\n",
    "\n",
    " Similarly,\n",
    " $$\n",
    " \\begin{aligned}\n",
    " \\frac{\\partial}{\\partial \\vec{\\beta}_2}\\left[\\frac{\\partial}{\\partial \\vec{\\beta}}log L\\right]^T = -\\sum_{i=1}^n\\left[-P(y_i=2|\\vec{x}_i)P(y_i=1|\\vec{x}_i) \\ \\ \\ \\ P(y_i=2|\\vec{x}_i)P(y_i\\neq2|\\vec{x}_i)\\right]\\otimes\\vec{x}_i.\\vec{x}_i^T\\end{aligned}$$\n",
    "\n",
    "So,\n",
    " $$\\begin{aligned}\n",
    " H &= \\begin{bmatrix}\\frac{\\partial}{\\partial \\vec{\\beta}_1} \\left[ \\frac{\\partial}{\\partial \\vec{\\beta}}log \\ L \\right]^T \\\\ \n",
    "    \\frac{\\partial}{\\partial \\vec{\\beta}_2} \\left[ \\frac{\\partial}{\\partial \\vec{\\beta}}log \\ L \\right]^T\n",
    "    \\end{bmatrix} \\\\ \n",
    "  \\\\ \n",
    "  &= \\begin{bmatrix}-\\sum_{i=1}^n\\left[P(y_i=1|\\vec{x}_i).P(y_i\\neq1|\\vec{x}_i) \\ \\ \\ \\ \\ \\ - P(y_i=1|\\vec{x}_i).P(y_i=2|\\vec{x}_i)\\right]\\otimes\\vec{x}_i.\\vec{x}_i^T \\\\ \n",
    "  -\\sum_{i=1}^n\\left[-P(y_i=2|\\vec{x}_i).P(y_i=1|\\vec{x}_i) \\ \\ \\ \\ \\ \\ \\ P(y_i=2|\\vec{x}_i).P(y_i\\neq2|\\vec{x}_i)\\right]\\otimes\\vec{x}_i.\\vec{x}_i^T\\end{bmatrix} \\\\ \n",
    "  \\\\ \n",
    "  &= -\\sum_{i=1}^n\\begin{bmatrix}P(y_i=1|\\vec{x}_i).P(y_i\\neq1|\\vec{x}_i) \\ \\ \\ \\ \\ - P(y_i=1|\\vec{x}_i).P(y_i=2|\\vec{x}_i) \\\\ \n",
    "  -P(y_i=2|\\vec{x}_i).P(y_i=1|\\vec{x}_i) \\ \\ \\ \\ \\ \\ P(y_i=2|\\vec{x}_i).P(y_i\\neq2|\\vec{x}_i)\n",
    "  \\end{bmatrix} \\otimes \\vec{x}_i.\\vec{x}_i^T\n",
    " \\end{aligned}\n",
    " $$\n",
    "\n",
    "To have unique maxima to the problem, $H$ has to be negative semi-definite, or $-H$ positive semi-definite. We can prove it in the following way.\n",
    "1.    Sum of positive definite matrices is positive definite. -H is sum of matrices. So, if we can show that the term inside sum is positive definite then -H is positive definite.\n",
    "2.    Kronecker Product of two positive semi-definite matrices is positive semi-definite. It follows from the following theory:  \n",
    "\n",
    "    **Theory:** Let, $\\mathbf{A_{mxm}}$ has eigen vectors **$\\mathbf{x_i}$** with corresponding eigen value $\\mathbf{\\lambda_i, i = 1, \\dots, m}$;  \n",
    "    $\\mathbf{B_{nxn}}$ has eighen vectors $\\mathbf{y_j}$ with corresponding eigen value $\\mathbf{\\mu_j, j = 1, \\dots n}$.  \n",
    "    Then, eigen vectors of $\\mathbf{A\\otimes B}$ is $\\mathbf{x_i \\otimes y_j}$ with corresponding eigen value $\\mathbf{\\lambda_i.\\mu_j}$.  \n",
    "    \n",
    "    **Proof:** Here, $Ax_i = \\lambda_i x_i$ and $By_j = \\mu_j y_j$. Now by the property (standard easily available on internet) of Kronecker Product $(A\\otimes B)(x_i\\otimes y_j) = (Ax_i)\\otimes (By_j)=(\\lambda_i x_i)\\otimes (\\mu_j y_j) = \\lambda_i\\mu_j(x_i\\otimes y_j)$. So, $x_i\\otimes y_j$ is the eigen vector corresponding to eigenvector $\\lambda_i\\mu_j$\n",
    "\n",
    "    Now, if **A** and **B** pd then both $\\lambda_i$ and $\\mu_j$ are non-negative. So is $\\lambda_i\\mu_j$, showing $A\\otimes B$ is positive semi-definite.\n",
    "\n",
    "    So if we can show that both the operands of the Kronecker Product is positve semi-definite, then -H will be postive semi-definite.\n",
    "3.    $\\vec{x}_i.\\vec{x}_i^T$ is positive semi-definite. We have to prove $\\begin{bmatrix}P(y_i=1|\\vec{x}_i).P(y_i\\neq1|\\vec{x}_i) \\ \\ \\ \\ \\ - P(y_i=1|\\vec{x}_i).P(y_i=2|\\vec{x}_i) \\\\ \n",
    "  -P(y_i=2|\\vec{x}_i).P(y_i=1|\\vec{x}_i) \\ \\ \\ \\ \\ \\ P(y_i=2|\\vec{x}_i).P(y_i\\neq2|\\vec{x}_i)\n",
    "  \\end{bmatrix}$ is positive semi-definite.\n",
    "\n",
    "  Now let,\n",
    "  $$\\begin{aligned}\n",
    "   P &= \\begin{bmatrix}\n",
    "   P(y_i=1|\\vec{x}_i).P(y_i\\neq1|\\vec{x}_i) \\ \\ \\ \\ \\ - P(y_i=1|\\vec{x}_i).P(y_i=2|\\vec{x}_i) \\\\ \n",
    "  -P(y_i=2|\\vec{x}_i).P(y_i=1|\\vec{x}_i) \\ \\ \\ \\ \\ \\ P(y_i=2|\\vec{x}_i).P(y_i\\neq2|\\vec{x}_i) \n",
    "  \\end{bmatrix} \\\\ \n",
    "   \\\\ \n",
    "   &= \\begin{bmatrix}\n",
    "   P(y_i=1|\\vec{x}_i).[1-P(y_i=1|\\vec{x}_i)] & - P(y_i=1|\\vec{x}_i).P(y_i=2|\\vec{x}_i) \\\\ \n",
    "  -P(y_i=2|\\vec{x}_i).P(y_i=1|\\vec{x}_i) & P(y_i=2|\\vec{x}_i).[1-P(y_i=2|\\vec{x}_i)]\n",
    "  \\end{bmatrix} \\\\ \n",
    "   \\\\\n",
    "   &= \\begin{bmatrix}\n",
    "   P(y_i=1|\\vec{x}_i)-P^2(y_i=1|\\vec{x}_i) & - P(y_i=1|\\vec{x}_i).P(y_i=2|\\vec{x}_i) \\\\ \n",
    "  -P(y_i=2|\\vec{x}_i).P(y_i=1|\\vec{x}_i) & P(y_i=2|\\vec{x}_i)-P^2(y_i=2|\\vec{x}_i)]\n",
    "  \\end{bmatrix} \\\\ \n",
    "   \\\\\n",
    "   &= \\begin{bmatrix}\n",
    "   P(y_i=1|\\vec{x}_i) & 0 \\\\ \n",
    "   0 & P(y_i=2|\\vec{x}_i)\n",
    "   \\end{bmatrix} - \n",
    "   \\begin{bmatrix}\n",
    "   P^2(y_i=1|\\vec{x}_i) & P(y_i=1|\\vec{x}_i).P(y_i=2|\\vec{x}_i) \\\\ \n",
    "   P(y_i=1|\\vec{x}_i).P(y_i=2|\\vec{x}_i) & P^2(y_i=2|\\vec{x}_i)\\end{bmatrix} \\\\ \n",
    "   \\\\ \n",
    "   &= \\begin{bmatrix}\n",
    "   P(y_i=1|\\vec{x}_i) & 0 \\\\ \n",
    "   0 & P(y_i=2|\\vec{x}_i)\n",
    "   \\end{bmatrix} - \n",
    "   \\begin{bmatrix}\n",
    "   P(y_i=1|\\vec{x}_i) \\\\ \n",
    "   P(y_i=2|\\vec{x}_i)\\end{bmatrix}.\n",
    "   \\begin{bmatrix}\n",
    "   P(y_i=1|\\vec{x}_i) \\\\ \n",
    "   P(y_i=2|\\vec{x}_i)\\end{bmatrix}^T\n",
    "   \\end{aligned}$$\n",
    "\n",
    "   So,\n",
    "   $$\\begin{aligned}\n",
    "   &  \\vec{z}^T.P.\\vec{z} \\\\ \n",
    "   &= \\vec{z}^T.\\begin{bmatrix}\n",
    "   P(y_i=1|\\vec{x}_i) & 0 \\\\ \n",
    "   0 & P(y_i=2|\\vec{x}_i)\n",
    "   \\end{bmatrix}.\\vec{z} - \\vec{z}^T.\n",
    "   \\begin{bmatrix}\n",
    "   P(y_i=1|\\vec{x}_i) \\\\ \n",
    "   P(y_i=2|\\vec{x}_i)\\end{bmatrix}.\n",
    "   \\begin{bmatrix}\n",
    "   P(y_i=1|\\vec{x}_i) \\\\ \n",
    "   P(y_i=2|\\vec{x}_i)\\end{bmatrix}^T.\\vec{z} \\\\ \n",
    "   \\\\\n",
    "   &= \\sum_{j=1}^2P(y_i=j|\\vec{x}_i)z_j^2 \\ \\ - \\ \\ \\left(\\sum_{j=1}^2P(y_i=j|\\vec{x}_i)z_j\\right)^2  \\end{aligned}$$\n",
    "\n",
    "Now, by **Cauchy-Schwarz Inequality**, $$\\left(\\sum_{j=1}^n u_jv_j\\right)^2 \\ \\ \\leq \\ \\ \\sum_{j=1}^n u_j^2.\\sum_{j=1}^nv_j^2$$\n",
    "\n",
    "If we set, n =2, $u_j=\\sqrt{P(y_i=j|\\vec{x}_i)}$ also as, $P(y_i=j|\\vec{x}_i) \\geq 0$, we can set $v_j=\\sqrt{P(y_i=j|\\vec{x}_i)}.z_j$; we get,\n",
    "$$\\begin{aligned}\n",
    " &\\left(\\sum_{j=1}^2 \\sqrt{P(y_i=j|\\vec{x}_i)}.\\sqrt{P(y_i=j|\\vec{x}_i)}.z_j\\right)^2 \\leq \\sum_{j=1}^2P(y_i=j|\\vec{x}_i).\\sum_{j=1}^2P(y_i=j|\\vec{x}_i).z_j^2 \\\\ \n",
    " \\implies & \\left(\\sum_{j=1}^2 P(y_i=j|\\vec{x}_i).z_j\\right)^2 \\leq \\sum_{j=1}^2P(y_i=j|\\vec{x}_i).z_j^2\n",
    "\\end{aligned}$$\n",
    "\n",
    "As, $\\sum_{j=1}^2P(y_i=j|\\vec{x}_i) = 1$.\n",
    "\n",
    "So, $\\vec{z}^T.P.\\vec{z} \\geq 0$. So, P is positive semi-definite.\n",
    "\n",
    "Using the above steps we can prove that -H is negative semi-definite, so H is positive semi-definite."
   ]
  }
 ],
 "metadata": {
  "colab": {
   "collapsed_sections": [],
   "name": "Multinomial_Logistic_Regression.ipynb",
   "provenance": []
  },
  "kernelspec": {
   "display_name": "Python 3 (ipykernel)",
   "language": "python",
   "name": "python3"
  },
  "language_info": {
   "codemirror_mode": {
    "name": "ipython",
    "version": 3
   },
   "file_extension": ".py",
   "mimetype": "text/x-python",
   "name": "python",
   "nbconvert_exporter": "python",
   "pygments_lexer": "ipython3",
   "version": "3.8.10"
  }
 },
 "nbformat": 4,
 "nbformat_minor": 5
}
